Actually, the typeclasses don't have to take the flag. Sorry @Theo

state/Compiler.STLC.fst
@@ -14,18 +14,18 @@ open BeyondCriteria
 
 noeq
 type src_interface1 = {
-  ct : fl:_ -> Type;
-  ct_targetlang : fl:_ -> targetlang fl default_spec (ct fl);
+  ct : Type;
+  ct_targetlang : targetlang default_spec ct;
 
   tct : typ;
-  _c : unit -> Lemma (elab_typ default_spec tct == ct All); (** can one even prove this? **)
+  _c : unit -> Lemma (elab_typ default_spec tct == ct); (** can one even prove this? **)
 }
 
-type ctx_src1 fl (i:src_interface1)  = i.ct fl
-type prog_src1 fl (i:src_interface1) = i.ct fl -> SST int (fun h0 -> True) (fun h0 _ h1 -> True)
+type ctx_src1 (i:src_interface1)  = i.ct
+type prog_src1 (i:src_interface1) = i.ct -> SST int (fun h0 -> True) (fun h0 _ h1 -> True)
 type whole_src1 = unit -> SST int (fun h0 -> True) (fun h0 _ h1 -> True)
 
-let link_src1 (#i:src_interface1) (p:prog_src1 All i) (c:ctx_src1 All i) : whole_src1 =
+let link_src1 (#i:src_interface1) (p:prog_src1 i) (c:ctx_src1 i) : whole_src1 =
   fun () -> p c
 
 val beh_src1 : whole_src1 ^-> st_mwp_h heap int
@@ -33,7 +33,7 @@ let beh_src1 = on_domain whole_src1 (fun ws -> theta (reify (ws ()))) (** what h
 
 let src_language1 : language (st_wp int) = {
   interface = src_interface1;
-  ctx = ctx_src1 All; pprog = prog_src1 All; whole = whole_src1;
+  ctx = ctx_src1; pprog = prog_src1; whole = whole_src1;
   link = link_src1;
   beh = beh_src1;
 }
@@ -84,7 +84,7 @@ let backtranslate_ctx1 #i ct =
   i._c ();
   instantiate_ctx_tgt1 ct
 
-val compile_pprog1 : (#i:src_interface1) -> prog_src1 All i -> prog_tgt1 (comp_int_src_tgt1 i)
+val compile_pprog1 : (#i:src_interface1) -> prog_src1 i -> prog_tgt1 (comp_int_src_tgt1 i)
 let compile_pprog1 #i ps =
   (fun c -> i._c (); ps c)
 
