state/TargetLang.fst
@@ -10,31 +10,31 @@ open Witnessable
 type targetlang_pspec =
   (inv:heap -> Type0) * (prref:mref_pred) * (hrel:FStar.Preorder.preorder heap)
 
-class targetlang (fl : erased tflag) (spec:targetlang_pspec) (t:Type) =
-  { wt : witnessable fl t }
+class targetlang (spec:targetlang_pspec) (t:Type) =
+  { wt : witnessable t }
 
-instance targetlang_unit pspec : targetlang All pspec unit = { wt = witnessable_unit }
-instance targetlang_int  pspec : targetlang All pspec int = { wt = witnessable_int }
-instance targetlang_pair pspec t1 t2 {| c1:targetlang All pspec t1 |} {| c2:targetlang All pspec t2 |}
-  : targetlang All pspec (t1 * t2)
+instance targetlang_unit pspec : targetlang pspec unit = { wt = witnessable_unit }
+instance targetlang_int  pspec : targetlang pspec int = { wt = witnessable_int }
+instance targetlang_pair pspec t1 t2 {| c1:targetlang pspec t1 |} {| c2:targetlang pspec t2 |}
+  : targetlang pspec (t1 * t2)
   = { wt = witnessable_pair t1 t2 #c1.wt #c2.wt }
-instance targetlang_univ_raise pspec (t1:Type u#a) {| c1:targetlang All pspec t1 |}
-  : targetlang All pspec (FStar.Universe.raise_t u#a u#b t1)
+instance targetlang_univ_raise pspec (t1:Type u#a) {| c1:targetlang pspec t1 |}
+  : targetlang pspec (FStar.Universe.raise_t u#a u#b t1)
   = { wt = witnessable_univ_raise t1 #c1.wt }
-instance targetlang_sum pspec t1 t2 {| c1:targetlang All pspec t1 |} {| c2:targetlang All pspec t2 |}
-  : targetlang All pspec (either t1 t2)
+instance targetlang_sum pspec t1 t2 {| c1:targetlang pspec t1 |} {| c2:targetlang pspec t2 |}
+  : targetlang pspec (either t1 t2)
   = { wt = witnessable_sum t1 t2 #c1.wt #c2.wt }
-instance targetlang_ref pspec t1 {| c1:targetlang All pspec t1 |}
-  : targetlang All pspec (ref t1)
+instance targetlang_ref pspec t1 {| c1:targetlang pspec t1 |}
+  : targetlang pspec (ref t1)
   = { wt = witnessable_mref t1 (FStar.Heap.trivial_preorder t1) #c1.wt }
-instance targetlang_llist pspec t1 {| c1:targetlang All pspec t1 |}
-  : targetlang All pspec (linkedList t1)
+instance targetlang_llist pspec t1 {| c1:targetlang pspec t1 |}
+  : targetlang pspec (linkedList t1)
   = { wt = witnessable_llist t1 #c1.wt }
 
 unfold let pre_targetlang_arrow
   (inv:heap -> Type0)
   (prref:mref_pred)
-  (#t1:Type) {| c1 : witnessable All t1 |}
+  (#t1:Type) {| c1 : witnessable t1 |}
   (x:t1) (h0:heap) =
   inv h0 /\ c1.satisfy x prref
 
@@ -42,21 +42,21 @@ unfold let post_targetlang_arrow
   (inv:heap -> Type0)
   (prref:mref_pred)
   (hrel:FStar.Preorder.preorder heap)
-  (#t1:Type) {| c1 : witnessable All t1 |}
-  (#t2:Type) {| c2 : witnessable All t2 |}
+  (#t1:Type) {| c1 : witnessable t1 |}
+  (#t2:Type) {| c2 : witnessable t2 |}
   (x:t1) (h0:heap) (r:t2) (h1:heap) =
   inv h1 /\ h0 `hrel` h1 /\ c2.satisfy r prref
 
 let mk_targetlang_arrow
   (pspec:targetlang_pspec)
-  (t1:Type) {| c1 : witnessable All t1 |}
-  (t2:Type) {| c2 : witnessable All t2 |}
+  (t1:Type) {| c1 : witnessable t1 |}
+  (t2:Type) {| c2 : witnessable t2 |}
 = x:t1 -> ST t2 All
     (requires (fun h0 -> (Mktuple3?._1 pspec) h0 /\ c1.satisfy x (Mktuple3?._2 pspec))) (** CA: super stupid that one has to use projectors **)
     (ensures (fun h0 r h1 -> (Mktuple3?._1 pspec) h1 /\ h0 `(Mktuple3?._3 pspec)` h1 /\ c2.satisfy r (Mktuple3?._2 pspec)))
 
-instance targetlang_arrow pspec t1 t2 {| c1:targetlang All pspec t1 |} {| c2:targetlang All pspec t2 |}
-  : targetlang All pspec (mk_targetlang_arrow pspec t1 #c1.wt t2 #c2.wt)
+instance targetlang_arrow pspec t1 t2 {| c1:targetlang pspec t1 |} {| c2:targetlang pspec t2 |}
+  : targetlang pspec (mk_targetlang_arrow pspec t1 #c1.wt t2 #c2.wt)
   = { wt = witnessable_arrow t1 t2 _ _ _ }
 
 let default_spec : targetlang_pspec = (
